First draft of request-response functions

src/lib/communication/DY.Lib.Communication.API.Invariants.fst
@@ -5,8 +5,11 @@ open DY.Core
 open DY.Lib.Communication.Core.Extension
 open DY.Lib.Crypto.PkEncryption.Split
 open DY.Lib.Crypto.Signature.Split
+open DY.Lib.Crypto.AEAD.Split
 open DY.Lib.Event.Typed
 open DY.Lib.State.PrivateKeys
+open DY.Lib.State.Tagged
+open DY.Lib.State.Typed
 
 open DY.Lib.Communication.API
 
@@ -30,6 +33,38 @@ val pkenc_crypto_predicates_communication_layer_and_tag:
   (string & pkenc_crypto_predicate)
 let pkenc_crypto_predicates_communication_layer_and_tag #cusages = 
   (comm_layer_pkenc_tag, pkenc_crypto_predicates_communication_layer)
+
+(*** AEAD Predicate ***)
+
+#push-options "--ifuel 1 --fuel 0"
+val aead_crypto_predicate_communication_layer: {|cusages:crypto_usages|} -> aead_crypto_predicate
+let aead_crypto_predicate_communication_layer #cusages = {
+  pred = (fun tr key_usage nonce msg ad ->
+    (match parse response_message msg with
+    | None -> False
+    | Some {id; payload} -> (
+      match parse authenticated_data ad with
+      | None -> False
+      | Some {client; server} -> (
+        event_triggered tr server (CommServerReceiveRequest server id payload) /\
+        (get_label tr id) `can_flow tr` (comm_label client server) /\
+        (get_label tr payload) `can_flow tr` (comm_label client server)
+      )
+    ))
+  );
+  pred_later = (fun tr1 tr2 key_usage nonce msg ad -> (
+    parse_wf_lemma response_message (bytes_well_formed tr1) msg;
+    parse_wf_lemma authenticated_data (bytes_well_formed tr1) ad;
+    ()
+  ))
+}
+#pop-options
+
+val aead_crypto_predicates_communication_layer_and_tag:
+  {|cusages:crypto_usages|} ->
+  (string & aead_crypto_predicate)
+let aead_crypto_predicates_communication_layer_and_tag #cusages =
+  (comm_layer_aead_tag, aead_crypto_predicate_communication_layer)
 
 (*** Sign Predicates ***)
 
@@ -64,12 +99,59 @@ val sign_crypto_predicates_communication_layer_and_tag:
 let sign_crypto_predicates_communication_layer_and_tag #cusages =
   (comm_layer_sign_tag, sign_crypto_predicates_communication_layer)
 
-val has_communication_layer_invariants:
+val has_communication_layer_crypto_predicates:
   {|crypto_invariants|} ->
   prop
-let has_communication_layer_invariants #cinvs =
+let has_communication_layer_crypto_predicates #cinvs =
   has_pkenc_predicate pkenc_crypto_predicates_communication_layer_and_tag /\
-  has_sign_predicate sign_crypto_predicates_communication_layer_and_tag
+  has_sign_predicate sign_crypto_predicates_communication_layer_and_tag /\
+  has_aead_predicate aead_crypto_predicates_communication_layer_and_tag
+
+
+(*** State Predicates ***)
+
+#push-options "--ifuel 2 --z3rlimit 25"
+let state_predicates_communication_layer {|crypto_invariants|}: local_state_predicate communication_states = {
+  pred = (fun tr prin sess_id st -> 
+    match st with
+    | ClientSendRequest {id; server; payload; key} -> (
+      let client = prin in
+      is_secret (comm_label client server) tr id /\
+      is_knowable_by (comm_label client server) tr payload /\
+      is_secret (comm_label client server) tr key
+    )
+    | ServerReceiveRequest {id; client; payload; key} -> (
+      let server = prin in
+      (exists client.
+        is_knowable_by (comm_label client server) tr id /\
+        is_knowable_by (comm_label client server) tr payload /\
+        is_knowable_by (comm_label client server) tr key
+      )
+    )
+    | ClientReceiveResponse {id; server; payload; key} -> (
+      let client = prin in
+      is_secret (comm_label client server) tr id /\
+      is_knowable_by (comm_label client server) tr payload /\
+      is_secret (comm_label client server) tr key
+    )
+  );
+  pred_later = (fun tr1 tr2 prin sess_id state -> ());
+  pred_knowable = (fun tr prin sess_id state -> ());
+}
+#pop-options
+
+val state_predicates_communication_layer_and_tag: 
+  {|crypto_invariants|} ->
+  dtuple2 string local_bytes_state_predicate
+let state_predicates_communication_layer_and_tag #cinvs =
+  (|local_state_communication_layer_session.tag, local_state_predicate_to_local_bytes_state_predicate (state_predicates_communication_layer #cinvs)|)
+
+val has_communication_layer_state_predicates:
+  {|protocol_invariants|} ->
+  prop
+let has_communication_layer_state_predicates #invs =
+  has_local_state_predicate state_predicates_communication_layer
+ 
 
 (*** Event Predicates ***)
 
@@ -108,6 +190,31 @@ type comm_higher_layer_event_preds = {
     )
     (ensures send_conf_auth tr2 sender receiver payload)
   ;
+  send_request: tr:trace -> client:principal -> server:principal -> payload:bytes -> prop;
+  send_request_later:
+    tr1:trace -> tr2:trace ->
+    client:principal -> server:principal -> payload:bytes ->
+    Lemma
+    (requires
+      send_request tr1 client server payload /\
+      tr1 <$ tr2
+    )
+    (ensures
+      send_request tr2 client server payload
+    )
+  ;
+  send_response: tr:trace -> server:principal -> payload:bytes -> prop;
+  send_response_later:
+    tr1:trace -> tr2:trace ->
+    server:principal -> payload:bytes ->
+    Lemma
+    (requires
+      send_response tr1 server payload /\
+      tr1 <$ tr2
+    )
+    (ensures
+      send_response tr2 server payload
+    )
 }
 
 val default_comm_higher_layer_event_preds: comm_higher_layer_event_preds
@@ -118,15 +225,24 @@ let default_comm_higher_layer_event_preds = {
   send_auth_later = (fun tr1 tr2 sender payload -> ());
   send_conf_auth = (fun tr sender receiver payload -> True);
   send_conf_auth_later = (fun tr1 tr2 sender receiver payload -> ());
+  send_request = (fun tr client server payload -> True);
+  send_request_later = (fun tr1 tr2 client server payload -> ());
+  send_response = (fun tr server payload -> True);
+  send_response_later = (fun tr1 tr2 server payload -> ())
 }
 
 #push-options "--ifuel 1 --fuel 0"
-let event_predicate_communication_layer {|cinvs:crypto_invariants|} (higher_layer_preds:comm_higher_layer_event_preds) : event_predicate communication_event =
+let event_predicate_communication_layer 
+  {|cinvs:crypto_invariants|}
+  (local_extension:comm_higher_layer_event_preds)
+  (higher_layer_preds:comm_higher_layer_event_preds) : 
+  event_predicate communication_event =
   fun tr prin e ->
     (match e with
     | CommConfSendMsg sender receiver payload -> (
       is_knowable_by (join (principal_label sender) (principal_label receiver)) tr payload /\
-      higher_layer_preds.send_conf tr sender receiver payload
+      higher_layer_preds.send_conf tr sender receiver payload /\
+      local_extension.send_conf tr sender receiver payload
     )
     | CommConfReceiveMsg receiver payload -> (
       exists sender.
@@ -165,19 +281,39 @@ let event_predicate_communication_layer {|cinvs:crypto_invariants|} (higher_laye
       //    decrypted payload flows to the receiver and some unknown sender'.
       event_triggered tr sender (CommConfAuthSendMsg sender receiver payload) \/
       is_corrupt tr (long_term_key_label sender)
-    ))
+    )
+    | CommClientSendRequest client server id payload -> (
+      is_knowable_by (comm_label client server) tr payload /\
+      higher_layer_preds.send_request tr client server payload
+    )
+    | CommServerReceiveRequest server id payload -> (
+      exists client. is_knowable_by (comm_label client server) tr payload /\
+      (event_triggered tr client (CommClientSendRequest client server id payload) \/
+        is_publishable tr payload)
+    )
+    | CommServerSendResponse server id payload -> (
+      (exists client. is_knowable_by (comm_label client server) tr payload) /\
+      higher_layer_preds.send_response tr server payload
+    )
+    | CommClientReceiveResponse client server id payload key -> (
+      event_triggered tr server (CommServerReceiveRequest server id payload) \/
+      is_corrupt tr (long_term_key_label server)
+    )
+    )
 #pop-options
 
 val event_predicate_communication_layer_and_tag: 
   {|cinvs:crypto_invariants|} ->
   comm_higher_layer_event_preds ->
+  comm_higher_layer_event_preds ->
   (string & compiled_event_predicate)
-let event_predicate_communication_layer_and_tag #cinvs higher_layer_preds =
-  (event_communication_event.tag, compile_event_pred #communication_event (event_predicate_communication_layer #cinvs higher_layer_preds))
+let event_predicate_communication_layer_and_tag #cinvs local_extension higher_layer_preds =
+  (event_communication_event.tag, compile_event_pred #communication_event (event_predicate_communication_layer #cinvs local_extension higher_layer_preds))
 
 val has_communication_layer_event_predicates:
   {|protocol_invariants|} ->
   comm_higher_layer_event_preds ->
+  comm_higher_layer_event_preds ->
   prop
-let has_communication_layer_event_predicates #invs higher_layer_preds =
-  has_event_pred (event_predicate_communication_layer higher_layer_preds)
+let has_communication_layer_event_predicates #invs local_extension higher_layer_preds =
+  has_event_pred (event_predicate_communication_layer local_extension higher_layer_preds)
